# Introduction

## Finite differences

Finite-difference calculus is based on the manipulation of finite differences of analytic functions. To introduce the subject we consider the analytic function ``f(x)``. The finite difference of ``f(x+h)`` and ``f(x)`` is called the *forward difference* and is defined as 
```math
Δ f(x)=f(x+h)-f(x).
```
Here, ``Δ`` is called the *forward-difference operator*. Likewise one defines the *backward-difference operator* ``∇``, 
```math
∇ f(x)=f(x)-f(x-h).
```
We first focus on *forward differences*. The derivative of ``f(x)`` is given by 
```math
f^′(x)=\underset{h→0}{\mathrm{lim}}\,\frac{f(x+h)-f(x)}{h}=\underset{Δ x→0}{\mathrm{lim}}\,\frac{Δ f(x)}{Δ x},
```
where ``h ≡ Δx ≥ 0`` is the *difference interval*. Introducing the differential operator, ``f^′(x) ≡ Df(x)``, we have 
```math
D≡\frac{d}{dx}=\underset{Δ x→0}{\mathrm{lim}}\,\frac{Δ}{Δ x}=\underset{h→0}{\mathrm{lim}}\,\frac{Δ}{h}.
```
## Translation operators 

**Forward difference notation**

With regard to *forward differences* we rewrite the forward difference definition in the form of a *forward translation*,
```math
f(x+h)=(1+Δ)f(x),
```
where ``T≡(1+Δ)`` is the *forward translation operator*. This operator shifts the function over the infinitesimal interval ``h`` to larger values of ``x``. The translation operator can be expressed in terms of the differential operator as follows by Taylor expansion of ``f(x)`` about the point ``x``, 
```math
f(x± h)=(1± hD+\tfrac{1}{2}h^2D^2±\tfrac{1}{3!}h^3D^3+⋯)f(x)=e^{± hD}f(x).
```
Comparing the operator expression for the *forward* translation with the Taylor expansion we obtain, by formal inversion of the operator ``T``, an operator identity for the inverted translation operator ``T^{-1}``,    
```math
T≡(1+Δ)=e^{hD}\,\,\,⇒\,\,\,T^{-1}=e^{-hD}=(1+Δ)^{-1}.
```
With this procedure, the explicit dependence on ``h`` can be replaced by an implicit dependence on ``h`` through an expansion in powers of ``Δ`` ,
```math
f(x-h)=(1+Δ)^{-1}f(x)=(1-Δ+Δ^{2}-Δ^3+⋯)f(x).
```
By choosing the proper expansion order, ``f(x-h)`` can be approximated to any desired level of accuracy.

**Backward difference notation**

Likewise, for *backward differences*, we rewrite the backward-difference definition in the form 
```math
f(x-h)=(1-∇)f(x),
```
where ``B≡(1-∇)`` is the *backward translation operator*. Comparing this *backward* translation with the Taylor expansion we obtain, by formal inversion of the operator ``B``, an operator identity for the *forward* translation operator ``T``, 
```math
B≡(1-∇)=e^{-hD}=T^{-1}\,\,\,⇒\,\,\,T=e^{hD}=(1+∇)^{-1}.
```
Note how the *backward* translation operator was identified with the inverse *forward* translation operator, ``B=T^{-1}``. When using backward differences, the explicit dependence on ``h`` can be replaced by an implicit dependence on ``h`` through an expansion in powers of ``∇``, 
```math
f(x+h)=(1-∇)^{-1}f(x)=(1+∇+∇^{2}+∇^3+⋯)f(x).
```
By choosing the proper expansion order, ``f(x+h)`` can be approximated to any desired level of accuracy. 

